# functors and applicatives

But back to Haskell...

I've been going through the Functors/Applicative sections of `learnyouahaskell`
and it has been a ride understanding it. Fortunately, I hang out with some pretty
knowledgable people and they helped me along.

One of the parts I didn't understand the most was where the definition for `<*>`
for the `Applicative ((->) r)` instance. This was explained to me in this method:

1. Check the type of `<*>`

    ```haskell
    Prelude> :t <*>
    (<*>) :: Applicative f => f (a -> b) -> f a -> f b
    ```

2. In this case, `f` is `((->) r)` or `r ->` which gives

    ```haskell
    f (a -> b) -> f a -> f b
    => (r -> a -> b) -> (r -> a) -> (r -> b)
    ```

3. And now to define `f <*> g`

    ```haskell
    -- based on the type of <*> we know
    -- f :: (r -> a -> b)
    -- g :: (r -> a)
    -- we want to return (r -> b) so let's start with that
    \r -> b
    -- how can we get `b`? by filling out `f`
    \r -> f r a
    -- and one way to get `a` is by using `g`
    \r -> f r (g r)
    -- therefore
    f <*> g = \r -> f r (g r)
    ```

I did the above by hand and double checked the final answer so I assume this is
how you would derive the definition. Things like this make me wonder if there's
another definition out there that would satisfy the
`(r -> a -> b) -> (r -> a) ->(r -> b)` typing, but I'm told there's a proof out
there that shows the above is the only sensible definition.

I believe this is kind of stumbling upon the topic of free theorems. This is basically
the idea that for some types, there is only one function that satisfies the type.
I can only think of one off the top of my head which is `a -> a` whose function
is `id`.

And this brought me to thinking about how `deriving` works. That would be something
to look into in the future perhaps.
